\documentclass[hyperref, a4paper]{article}

\usepackage{geometry}
\usepackage{titling}
\usepackage{titlesec}
% No longer needed, since we will use enumitem package
% \usepackage{paralist}
\usepackage{enumitem}
\usepackage{footnote}
\usepackage{enumerate}
\usepackage{amsmath, amssymb, amsthm}
\usepackage{mathtools}
\usepackage{bbm}
\usepackage{cite}
\usepackage{graphicx}
\usepackage{subfigure}
\usepackage{physics}
\usepackage{tensor}
\usepackage{siunitx}
\usepackage[version=4]{mhchem}
\usepackage{tikz}
\usepackage{xcolor}
\usepackage{listings}
\usepackage{autobreak}
\usepackage[ruled, vlined, linesnumbered]{algorithm2e}
\usepackage{nameref,zref-xr}
\zxrsetup{toltxlabel}
\usepackage[colorlinks,unicode]{hyperref} % , linkcolor=black, anchorcolor=black, citecolor=black, urlcolor=black, filecolor=black
\usepackage[most]{tcolorbox}
\usepackage{prettyref}

% Page style
\geometry{left=3.18cm,right=3.18cm,top=2.54cm,bottom=2.54cm}
\titlespacing{\paragraph}{0pt}{1pt}{10pt}[20pt]
\setlength{\droptitle}{-5em}
\preauthor{\vspace{-10pt}\begin{center}}
\postauthor{\par\end{center}}

% More compact lists 
\setlist[itemize]{
    itemindent=17pt, 
    leftmargin=1pt,
    listparindent=\parindent,
    parsep=0pt,
}

% Math operators
\DeclareMathOperator{\timeorder}{\mathcal{T}}
\DeclareMathOperator{\diag}{diag}
\DeclareMathOperator{\legpoly}{P}
\DeclareMathOperator{\primevalue}{P}
\DeclareMathOperator{\sgn}{sgn}
\newcommand*{\ii}{\mathrm{i}}
\newcommand*{\ee}{\mathrm{e}}
\newcommand*{\const}{\mathrm{const}}
\newcommand*{\suchthat}{\quad \text{s.t.} \quad}
\newcommand*{\argmin}{\arg\min}
\newcommand*{\argmax}{\arg\max}
\newcommand*{\normalorder}[1]{: #1 :}
\newcommand*{\pair}[1]{\langle #1 \rangle}
\newcommand*{\fd}[1]{\mathcal{D} #1}
\DeclareMathOperator{\bigO}{\mathcal{O}}

% TikZ setting
\usetikzlibrary{arrows,shapes,positioning}
\usetikzlibrary{arrows.meta}
\usetikzlibrary{decorations.markings}
\tikzstyle arrowstyle=[scale=1]
\tikzstyle directed=[postaction={decorate,decoration={markings,
    mark=at position .5 with {\arrow[arrowstyle]{stealth}}}}]
\tikzstyle ray=[directed, thick]
\tikzstyle dot=[anchor=base,fill,circle,inner sep=1pt]

% Algorithm setting
% Julia-style code
\SetKwIF{If}{ElseIf}{Else}{if}{}{elseif}{else}{end}
\SetKwFor{For}{for}{}{end}
\SetKwFor{While}{while}{}{end}
\SetKwProg{Function}{function}{}{end}
\SetArgSty{textnormal}

\newcommand*{\concept}[1]{{\textbf{#1}}}

% Embedded codes
\lstset{basicstyle=\ttfamily,
  showstringspaces=false,
  commentstyle=\color{gray},
  keywordstyle=\color{blue}
}

% Reference formatting
\newrefformat{fig}{Figure~\ref{#1}}

% Color boxes
\tcbuselibrary{skins, breakable, theorems}
\newtcbtheorem[number within=section]{warning}{Warning}%
  {colback=orange!5,colframe=orange!65,fonttitle=\bfseries, breakable}{warn}
\newtcbtheorem[number within=section]{note}{Note}%
  {colback=green!5,colframe=green!65,fonttitle=\bfseries, breakable}{note}
\newtcbtheorem[number within=section]{info}{Info}%
  {colback=blue!5,colframe=blue!65,fonttitle=\bfseries, breakable}{info}

\newenvironment{shelldisplay}{\begin{lstlisting}}{\end{lstlisting}}

\title{Many-body Physics Homework 2}
\author{Jinyuan Wu}

\begin{document}

\maketitle

\paragraph{Problem 1}

\paragraph{Solution} \begin{itemize}
\item[1.] We make the Trotter decomposition:
\begin{equation}
    \begin{aligned}
        \mel{\alpha_f}{\ee^{- \ii H(t_f - t_i)}}{\alpha_i} &= \lim_{N \to \infty}
        \prod_{j=1}^{N-1} \int \frac{\dd{\alpha_j}}{\pi} \prod_{j=1}^N \mel{\alpha_j}{\ee^{- \ii \Delta t H}}{\alpha_{j-1}} \\
        &= \lim_{N\to \infty} \prod_{j=1}^{N-1} \int \frac{\dd{\alpha_j}}{\pi} \prod_{j=1}^N 
        \ee^{- \ii \Delta t \omega \alpha_{j-1}^* \alpha_{j-1}} \braket*{\alpha_j}{\alpha_{j-1}} \\
        &= \lim_{N \to \infty} \prod_{j=1}^{N-1} \int \frac{\dd{\alpha_j}}{\pi} \prod_{j=1}^N 
        \ee^{- \ii \Delta t \omega \alpha_{j-1}^* \alpha_{j-1}}
        \ee^{- \frac{1}{2} (\abs{\alpha_j}^2 + \abs{\alpha_{j-1}}^2) + \alpha_j^* \alpha_{j-1}} ,
    \end{aligned}
\end{equation}
where $\Delta \tau = (t_f - t_i) / N$, $\alpha_N = \alpha_f$,
and $\alpha_0 = \alpha_i$.

\item[2.] To continue, we can use the condition that $\alpha_j$ and $\alpha_{j-1}$ is close to each other 
and make the following derivation: 
\[
    \begin{aligned}
        \mel{\alpha_f}{\ee^{- \ii H(t_f - t_i)}}{\alpha_i} 
        &= \lim_{N \to \infty} \prod_{j=1}^{N-1} \int \frac{\dd{\alpha_j}}{\pi} \prod_{j=1}^N 
        \ee^{- \ii \Delta t \omega \alpha_{j-1}^* \alpha_{j-1}}
        \ee^{- \alpha^*_j \alpha_j + \alpha_j^* \alpha_{j-1}} \\ 
        &= \lim_{N \to \infty} \prod_{j=1}^{N-1} \int \frac{\dd{\alpha_j}}{\pi} \prod_{j=1}^N 
        \ee^{- \ii \Delta t \omega \alpha_{j-1}^* \alpha_{j-1} - \alpha_j^* (\alpha_j - \alpha_{j-1})} \\
        &= \lim_{N \to \infty} \prod_{j=1}^{N-1} \int \frac{\dd{\alpha_j}}{\pi} \prod_{j=1}^N 
        \ee^{\ii \Delta t (\ii \alpha_j^* (\alpha_j - \alpha_{j-1}) / \Delta t - \omega \alpha_{j-1}^* \alpha_{j-1}) } \\
        &= \lim_{N \to \infty} \left( \prod_{j=1}^{N-1} \int \frac{\dd{\alpha_j}}{\pi} \right)
        \ee^{\ii \sum_j \Delta t (\ii \alpha_j^* (\alpha_j - \alpha_{j-1}) / \Delta t - \omega \alpha_{j-1}^* \alpha_{j-1}) },
    \end{aligned}
\]
so after taking the continuous limit, we get 
\begin{equation}
    \mel{\alpha_f}{\ee^{- \ii H (t_f - t_i)}}{\alpha_i} = \int \mathcal{D} \alpha 
    \ee^{\ii \int_{t_i}^{t_f} \dd{t} (\ii \alpha^* \dot{\alpha} - \omega \abs{\alpha}^2 )}.
\end{equation}
So the Lagrangian is 
\begin{equation}
    L = \ii \alpha^* \dot{\alpha} - \omega \abs{\alpha}^2.
    \label{eq:lagrangian-oscillator}
\end{equation}

\item[3.] By putting 
\begin{equation}
    \alpha = \sqrt{\frac{m \omega}{2}} (x + \ii p / m \omega) 
\end{equation}
into \eqref{eq:lagrangian-oscillator}, we get 
\[
    \begin{aligned}
        L &= \ii \frac{m \omega}{2} \left( x - \frac{\ii p}{m \omega} \right) 
        \left( \dot{x} + \frac{\ii \dot{p}}{m \omega} \right) 
        - \omega \frac{m \omega}{2} \left( x - \frac{\ii p}{m \omega} \right) 
        \left( x + \frac{\ii p}{m \omega} \right) \\
        &= \ii \frac{m \omega}{2} \left( x - \frac{\ii p}{m \omega} \right) 
        \left( \dot{x} + \frac{\ii \dot{p}}{m \omega} \right) 
        - \frac{p^2}{2m} - \frac{1}{2} m \omega^2 x^2.
    \end{aligned}
\]
By integration by parts, we have 
\[
    \dot{p} \left( x - \frac{\ii p}{m \omega} \right) 
    = \dv{t} \left( px - \frac{\ii p^2}{m \omega} \right) 
    - p \left( \dot{x} - \frac{\ii \dot{p}}{m \omega} \right),
\]
and thus 
\[
    \begin{aligned}
        &\quad \ii \frac{m \omega}{2} \left( x - \frac{\ii p}{m \omega} \right) 
        \left( \dot{x} + \frac{\ii \dot{p}}{m \omega} \right) \\
        &= \ii \frac{m \omega}{2} \left( x \dot{x} - \frac{\ii}{m \omega} p \dot{x} + \frac{\ii}{m \omega} \left( \dv{t} \left( px - \frac{\ii p^2}{m \omega} \right) 
        - p \left( \dot{x} - \frac{\ii \dot{p}}{m \omega} \right) \right) \right) \\
        &= \frac{\ii m \omega}{2} \left( - \frac{2 \ii}{m \omega} p \dot{x} + 
        \dv{t} \left( x^2 - \frac{p^2}{m^2 \omega^2} \right) \right) \\
        &= p \dot{x} + \text{total time derivative}.
    \end{aligned}
\]
So we have 
\begin{equation}
    L = p \dot{x} - \frac{p^2}{2m} - \frac{1}{2} m \omega^2 x^2 + \text{total time derivative}.
\end{equation}

\end{itemize}

\paragraph{Problem 2} 

\paragraph{Solution} \begin{itemize}
\item[1.] The discrete path integral is 
\[
    \begin{aligned}
        \mel{\vb*{x}_f}{\ee^{- \ii H t}}{\vb*{x}_i} &= 
        \lim_{N \to \infty} \prod_{j=1}^{N-1} \int \dd[3]{\vb*{x}_j} 
        \prod_{j=1}^N \mel{\vb*{x}_j}{\ee^{- \ii \Delta t H}}{\vb*{x}_{j-1}} \\
        &= \lim_{N \to \infty} \prod_{j=1}^{N-1} \int \dd[3]{\vb*{x}_j} 
        \prod_{j=1}^N \mel{\vb*{x}_j}{\ee^{- \ii \Delta t ( 
            \hat{\vb*{p}}^2  - \hat{\vb*{p}} \cdot \vb*{A}(\vb*{x}_{j-1}) 
            - \vb*{A}(\vb*{x}_j) \cdot \hat{\vb*{p}} + \vb*{A}(\vb*{x}_{j-1})^2
        ) / 2m}}{\vb*{x}_{j-1}}.
    \end{aligned}
\]
Now we introduce a $\vb*{p}$ variable to eliminate the momentum operator:
\[
    \begin{aligned}
        &\quad \mel{\vb*{x}_j}{\ee^{- \ii \Delta t ( 
            \hat{\vb*{p}}^2  - \hat{\vb*{p}} \cdot \vb*{A}(\vb*{x}_{j-1}) 
            - \vb*{A}(\vb*{x}_j) \cdot \hat{\vb*{p}} + \vb*{A}(\vb*{x}_{j-1})^2
        ) / 2m}}{\vb*{x}_{j-1}} \\
        &= \int \dd[3]{\vb*{p}} \braket*{\vb*{x}_j}{\vb*{p}}
        \mel{\vb*{p}}{\ee^{- \ii \Delta t ( 
            \hat{\vb*{p}}^2  - \hat{\vb*{p}} \cdot \vb*{A}(\vb*{x}_{j-1}) 
            - \vb*{A}(\vb*{x}_j) \cdot \hat{\vb*{p}} + \vb*{A}(\vb*{x}_{j-1})^2
        ) / 2m}}{\vb*{x}_{j-1}} \\
        &= \int \frac{\dd[3]{\vb*{p}}}{(2\pi)^3} \ee^{\ii \vb*{p} \cdot \vb*{x}_j}
        \ee^{- \ii \Delta t ( 
            {\vb*{p}}^2  - {\vb*{p}} \cdot \vb*{A}(\vb*{x}_{j-1}) 
            - \vb*{A}(\vb*{x}_j) \cdot {\vb*{p}} + \vb*{A}(\vb*{x}_{j-1})^2
        ) / 2m}
        \ee^{- \ii \vb*{p} \cdot \vb*{x}_{j-1}} \\
        &= \ee^{- \ii \Delta t \vb*{A}(\vb*{x}_{j-1})^2 / 2m} 
        \int \frac{\dd[3]{\vb*{p}}}{(2\pi)^3} \ee^{- \frac{1}{2} \frac{\ii \Delta t}{m} \vb*{p}^2}
        \ee^{\ii \vb*{p} \cdot \left(
            \vb*{x}_j - \vb*{x}_{j-1} +
            \frac{\Delta t}{2m} (\vb*{A} (\vb*{x}_j) + \vb*{A}(\vb*{x}_{j-1}) )
        \right)} \\
        &= \ee^{- \ii \Delta t \vb*{A}(\vb*{x}_{j-1})^2 / 2m} \frac{1}{(2\pi)^3} \sqrt{\frac{(2\pi)^3}{(\ii \Delta t / m)^3}} \ee^{- \frac{1}{2} \frac{m}{\ii \Delta t} \left(
            \vb*{x}_j - \vb*{x}_{j-1} +
            \frac{\Delta t}{2m} (\vb*{A} (\vb*{x}_j) + \vb*{A}(\vb*{x}_{j-1}) )
        \right)^2 } \\
        &\approx \sqrt{\frac{- \ii m^3}{(2\pi)^3 \Delta t^3}} \ee^{\ii \Delta t \frac{m}{2} 
        \left(\frac{(\vb*{x}_j - \vb*{x}_{j-1})^2}{\Delta t^2} 
        + \frac{\vb*{x}_j - \vb*{x}_{j-1}}{\Delta t} \cdot \frac{\vb*{A}(\vb*{x}_j) + \vb*{A}(\vb*{x}_{j-1})}{2}\right)}.
    \end{aligned}
\]
Here in the last line we make the approximation that $\vb*{A}(\vb*{x}_j)$ and $\vb*{A}(\vb*{x}_{j-1})$
are close to each other,
so the two $\vb*{A}^2$ terms cancel with each other.
So the final discrete path integral is 
\begin{equation}
    \begin{aligned}
        \mel{\vb*{x}_f}{\ee^{- \ii H t}}{\vb*{x}_i} &= 
        \lim_{N \to \infty} \prod_{j=1}^{N-1} \left( \frac{- \ii m^3}{(2\pi)^3 \Delta t^3} \right)^{N/2}
        \int \dd[3]{\vb*{x}_j} \\
        &\quad \quad \cdot \ee^{\sum_{j=1}^N \ii \Delta t 
            \left( \frac{m}{2}  \frac{(\vb*{x}_j - \vb*{x}_{j-1})^2}{\Delta t^2} 
            + \frac{\vb*{x}_j - \vb*{x}_{j-1}}{\Delta t} \cdot \frac{\vb*{A}(\vb*{x}_j) + \vb*{A}(\vb*{x}_{j-1})}{2}\right)}.
    \end{aligned}
    \label{eq:magnetic-path-integral-1}
\end{equation}

\item[2.] The derivation is largely the same, but now in each time stp,
the $- 2 \hat{\vb*{p}} \cdot \vb*{A}(\vb*{x})$ term 
results in $- 2 \hat{\vb*{p}} \cdot \vb*{A}(\vb*{x}_{j-1})$,
and the result is 
\begin{equation}
    \begin{aligned}
        \mel{\vb*{x}_f}{\ee^{- \ii H t}}{\vb*{x}_i} &= 
        \lim_{N \to \infty} \prod_{j=1}^{N-1} \left( \frac{- \ii m^3}{(2\pi)^3 \Delta t^3} \right)^{N/2}
        \int \dd[3]{\vb*{x}_j} \\
        &\quad \quad \cdot \ee^{\sum_{j=1}^N \ii \Delta t 
            \left(\frac{m}{2} \frac{(\vb*{x}_j - \vb*{x}_{j-1})^2}{\Delta t^2} 
            + \frac{\vb*{x}_j - \vb*{x}_{j-1}}{\Delta t} \cdot \vb*{A}(\vb*{x}_{j-1}) + \frac{\ii}{2m} \div{\vb*{A} (\vb*{x}_{j-1})} \right)}.
    \end{aligned}
    \label{eq:magnetic-path-integral-2}
\end{equation}

\item[3.] We make the following replacements:
\[
    \frac{(\vb*{x}_j - \vb*{x}_{j-1})^2}{\Delta t^2} \longrightarrow \dot{\vb*{x}}^2, \quad 
    \sum_j \Delta t = \int \dd{t},
\]
and from \eqref{eq:magnetic-path-integral-1} we get 
\begin{equation}
    \mel{\vb*{x}_f}{\ee^{- \ii H t}}{\vb*{x}_i} = \int \fd{\vb*{x}} \ee^{\ii \int_{t_i}^{t_f} \dd{t}
    \left(  \frac{1}{2} m \dot{\vb*{x}}^2 + \dot{\vb*{x}} \cdot \vb*{A}\right) },
\end{equation} 
and from \eqref{eq:magnetic-path-integral-2} we get 
\begin{equation}
    \mel{\vb*{x}_f}{\ee^{- \ii H t}}{\vb*{x}_i} = \int \fd{\vb*{x}} \ee^{\ii \int_{t_i}^{t_f} \dd{t}
    \left(  \frac{1}{2} m \dot{\vb*{x}}^2 + \dot{\vb*{x}} \cdot \vb*{A} + \frac{\ii}{2m} \div{\vb*{A}} \right) }.
\end{equation}
So for the first path integral the Lagrangian is 
\begin{equation}
    L = \frac{1}{2} m \dot{\vb*{x}}^2 + \dot{\vb*{x}} \cdot \vb*{A},
\end{equation}
while for the second, it is 
\begin{equation}
    L = \frac{1}{2} m \dot{\vb*{x}}^2 + \dot{\vb*{x}} \cdot \vb*{A} + \frac{\ii}{2m} \div{\vb*{A}}.
\end{equation}

\item[4.] 

\end{itemize}

\paragraph{Problem 3}

\paragraph{Solution} 

\paragraph{Problem 4} 

\paragraph{Solution} \begin{itemize}
\item[1.] We do the Trotter decomposition again:
\[
    \mel{\vb*{k}_f}{\ee^{- \ii H t}}{\vb*{k}_i} = \lim_{N \to \infty}
    \prod_{j=1}^{N-1} \int \frac{V}{(2\pi)^3} \dd[3]{\vb*{k}_j} \cdot \prod_{j=1}^{N} 
    \mel{\vb*{k}_j}{\ee^{- \ii \Delta t H}}{\vb*{k}_{j-1}}, \quad 
    \vb*{k}_{0} = \vb*{k}_i, \quad \vb*{k}_N = \vb*{k}_f.
\]
Each time step is given by 
\[
    \begin{aligned}
        &\quad \mel{\vb*{k}_j}{\ee^{- \ii \Delta t (H_0 + \hat{\vb*{x}}^2 / 2 \alpha - \vb*{E} \cdot \hat{\vb*{x}})}}{\vb*{k}_{j-1}} \\
        &= \mel{\vb*{k}_j}{\ee^{- \ii \Delta t ( \hat{\vb*{x}}^2 / 2 \alpha - \vb*{E} \cdot \hat{\vb*{x}})}}{\vb*{k}_{j-1}} \ee^{- \Delta t \epsilon_{\vb*{k}_{j-1}}} \\
        &= \ee^{- \Delta t \epsilon_{\vb*{k}_{j-1}}} \int \dd[3]{\vb*{r}} u^*_{\vb*{k}_j}(\vb*{r}) \ee^{- \ii \vb*{k}_j \cdot \vb*{r}}
        \ee^{- \ii \Delta t (\vb*{r}^2 / 2\alpha - \vb*{E} \cdot \vb*{r})} u_{\vb*{k}_{j-1}}(\vb*{r}) \ee^{\ii \vb*{k}_{j-1} \cdot \vb*{r}} \\
        &= \ee^{- \Delta t \epsilon_{\vb*{k}_{j-1}}} \int \dd[3]{\vb*{r}} u^*_{\vb*{k}_{j}}(\vb*{r}) u_{\vb*{k}_{j-1}}(\vb*{r})
        \ee^{- \frac{1}{2} \frac{\ii \Delta t}{\alpha} \vb*{r}^2 + \ii \vb*{r} \cdot (\Delta t \vb*{E} + \vb*{k}_{j-1} - \vb*{k}_j) }.
    \end{aligned}
\]
The semi-classical dynamics only works when $\psi_{\vb*{k}}(\vb*{r})$ is 
``concentrated'' enough in the reciprocal space,
which means $u_{\vb*{k}}(\vb*{r})$ should be very smooth compared with $\ee^{\ii \vb*{k} \cdot \vb*{r}}$
(or otherwise the picture of an electron with a certain momentum traveling in the material is simply wrong).
Thus, we have 
\[
    \begin{aligned}
        &\quad \int \dd[3]{\vb*{r}} u^*_{\vb*{k}_{j}}(\vb*{r}) u_{\vb*{k}_{j-1}}(\vb*{r})
        \ee^{- \frac{1}{2} \frac{\ii \Delta t}{\alpha} \vb*{r}^2 + \ii \vb*{r} \cdot (\Delta t \vb*{E} + \vb*{k}_{j-1} - \vb*{k}_j) } \\
        &= \frac{1}{V_{\text{u.c.}}} \int_{\text{u.c.}} \dd[3]{\vb*{r}}
        u^*_{\vb*{k}_{j}}(\vb*{r}) u_{\vb*{k}_{j-1}}(\vb*{r})
        \int \dd[3]{\vb*{r}} \ee^{- \frac{1}{2} \frac{\ii \Delta t}{\alpha} \vb*{r}^2 + \ii \vb*{r} \cdot (\Delta t \vb*{E} + \vb*{k}_{j-1} - \vb*{k}_j) } ,
    \end{aligned}
\]
and the Gaussian integral on the RHS can be evaluated as 
\[
    \begin{aligned}
        &\int \dd[3]{\vb*{r}} \ee^{- \frac{1}{2} \frac{\ii \Delta t}{\alpha} \vb*{r}^2 + \ii \vb*{r} \cdot (\Delta t \vb*{E} + \vb*{k}_{j-1} - \vb*{k}_j) }  \\
        &= \sqrt{\frac{(2\pi)^3}{(\ii \Delta t / \alpha)^3}} \ee^{\frac{1}{2} \frac{\alpha}{\ii \Delta t} (\ii (\Delta t \vb*{E} + \vb*{k}_{j-1} - \vb*{k}_j))^2 } \\
        &= \sqrt{\frac{(2\pi)^3}{(\ii \Delta t / \alpha)^3}} \ee^{ \frac{\ii \alpha}{2} (\vb*{E} - \dot{\vb*{k}})^2 \Delta t }.
    \end{aligned}
\]
Thus 
\[
    \begin{aligned}
        \mel{\vb*{k}_f}{\ee^{- \ii H t}}{\vb*{k}_i} &= \lim_{N \to \infty} \mathcal{N} \prod_{j=1}^{N-1} 
        \int \dd[3]{\vb*{k}_j} \ee^{- \ii \Delta t \epsilon_{\vb*{k}_{j-1}}} \ee^{\frac{\ii \Delta t \alpha}{2} (\dot{\vb*{k}} - \vb*{E})^2}
        \braket*{u_{\vb*{k}_j}}{u_{\vb*{k}_{j-1}}} \\
        &= \lim_{N \to \infty} \mathcal{N} \prod_{j=1}^{N-1} 
        \int \dd[3]{\vb*{k}_j} \ee^{- \ii \Delta t \epsilon_{\vb*{k}_{j-1}}} \ee^{\frac{\ii \Delta t \alpha}{2} (\dot{\vb*{k}} - \vb*{E})^2}
        (1 - \Delta t \dot{\vb*{k}} \cdot \mel*{u_{\vb*{k}_{j}}}{\grad_{\vb*{k}_{j}}}{u_{\vb*{k}_{j}}}) \\
        &= \lim_{N \to \infty} \mathcal{N} \prod_{j=1}^{N-1} 
        \int \dd[3]{\vb*{k}_j} \ee^{- \ii \Delta t \epsilon_{\vb*{k}_{j-1}} + \frac{\ii \Delta t \alpha}{2} (\dot{\vb*{k}} - \vb*{E})^2 - \Delta t \dot{\vb*{k}} \cdot \mel*{u_{\vb*{k}_{j}}}{\grad_{\vb*{k}_{j}}}{u_{\vb*{k}_{j}}}} \\
        &= \lim_{N \to \infty}  \left(\mathcal{N} \prod_{j=1}^{N-1} 
        \int \dd[3]{\vb*{k}_j}\right) \ee^{\ii \Delta t (\sum_{j} - \epsilon_{\vb*{k}_{j-1}} + \frac{ \alpha}{2} (\dot{\vb*{k}} - \vb*{E})^2 + \ii \dot{\vb*{k}} \cdot \mel*{u_{\vb*{k}_{j}}}{\grad_{\vb*{k}_{j}}}{u_{\vb*{k}_{j}}})}.
    \end{aligned}
\]
Putting all normalization factors into the measure, we get 
\begin{equation}
    \begin{aligned}
        \mel{\vb*{k}_f}{\ee^{- \ii H t}}{\vb*{k}_i} = \int \mathcal{D} \vb*{k} \ee^{\ii \int_i^f \dd{t} L_{\text{eff}}}, \\
        L_{\text{eff}} = \dot{\vb*{k}} \cdot \vb*{\mathcal{A}} + \frac{\alpha}{2} (\dot{\vb*{k}} - \vb*{E})^2 - \epsilon_{\vb*{k}}.
    \end{aligned}
\end{equation}
So we find 
\begin{equation}
    \mathcal{F}(\vb*{k}, \dot{\vb*{k}}) = \frac{\alpha}{2} (\dot{\vb*{k}} - \vb*{E})^2 - \epsilon_{\vb*{k}}.
\end{equation}

\item[2.] We have 
\begin{equation}
    \vb*{\pi} = \pdv{L_{\text{eff}}}{\dot{\vb*{k}}} = \vb*{\mathcal{A}} + \alpha (\dot{\vb*{k}} - \vb*{E}).
\end{equation}
So 
\[
    \begin{aligned}
        H_{\text{eff}} &= \dot{\vb*{k}} \cdot \vb*{\pi} - L_{\text{eff}} \\
        &= \frac{1}{2} \alpha \dot{\vb*{k}}^2 - \frac{1}{2} \alpha \vb*{E}^2 + \epsilon_{\vb*{k}}.
    \end{aligned}
\]
Replacing $\dot{\vb*{k}}$ by $\vb*{\pi}$, 
we get 
\[
    \begin{aligned}
        H_{\text{eff}} &= \frac{1}{2} \alpha \left( \frac{\vb*{\pi} - \vb*{\mathcal{A}}}{\alpha} + \vb*{E} \right)^2
        - \frac{1}{2} \alpha \vb*{E}^2 + \epsilon_{\vb*{k}} \\
        &= \frac{(\vb*{\pi} - \vb*{\mathcal{A}})^2}{2 \alpha} + (\vb*{\pi} - \vb*{\mathcal{A}}) \cdot \vb*{E} + \epsilon_{\vb*{k}}.
    \end{aligned}
\]
So the answer is 
\begin{equation}
    H_{\text{eff}} = \frac{(\vb*{\pi} - \vb*{\mathcal{A}})^2}{2 \alpha} + (\vb*{\pi} - \vb*{\mathcal{A}}) \cdot \vb*{E} + \epsilon_{\vb*{k}}.
\end{equation}

\item[3.] We can interpret $-\vb*{\pi}$ as some sort of ``position'',
because 
\[
    \comm{\vb*{k}}{\vb*{\pi}} = 1 \Leftrightarrow \comm{- \vb*{\pi}}{\vb*{k}} = 1,
\]
so we replace $\vb*{\pi}$ by $- \vb*{x}$, and thus in the $\alpha \to \infty$ limit, we have
\begin{equation}
    H_{\text{eff}} = - (\vb*{x} + \vb*{\mathcal{A}}) \cdot \vb*{E} + \epsilon_{\vb*{k}}.
\end{equation}

\item[4.] We have 
\[
    \dot{\vb*{x}} = \pdv{H_{\text{eff}}}{\vb*{k}} = \grad_{\vb*{k}} \epsilon_{\vb*{k}} - \grad_{\vb*{k}} (\vb*{E} \cdot \vb*{\mathcal{A}}).
\]
By vector analysis formula, and by the condition that $\vb*{E}$ is a constant,
we have 
\[
    \grad_{\vb*{k}} (\vb*{E} \cdot \mathcal{\vb*{A}}) = \vb*{E} \times (\grad_{\vb*{k}} \times \vb*{\mathcal{A}}),
\]
so finally we get
\begin{equation}
    \dot{\vb*{x}} = \grad_{\vb*{k}} \epsilon_{\vb*{k}} - \vb*{E} \times \vb*{\Omega},
    \label{eq:x-eom}
\end{equation}
where 
\begin{equation}
    \vb*{\Omega} = \grad_{\vb*{k}} \times \vb*{\mathcal{A}}.
\end{equation}
Also 
\begin{equation}
    \dot{\vb*{k}} = - \pdv{H_{\text{eff}}}{\vb*{x}} = \vb*{E}.
    \label{eq:k-eom}
\end{equation}

\item[5.] From \eqref{eq:x-eom} and \eqref{eq:k-eom} we have%
\footnote{
    Here we assume there is a very weak electric field $\vb*{E}$,
    so we can put \eqref{eq:k-eom} and \eqref{eq:x-eom} into one equation,
    and then we let $\vb*{E} \to 0$.
}
\[
    \dot{\vb*{x}} = - \vb*{E} \times \vb*{\Omega} = - \dot{\vb*{k}} \times \vb*{\Omega}, 
\]
and therefore 
\begin{equation}
    \vb*{\Omega} \times \dot{\vb*{x}} = - \Omega^2 \dot{\vb*{k}} + (\vb*{\Omega} \cdot \dot{\vb*{k}}) \vb*{\Omega}.
    \label{eq:eom-iqhe}
\end{equation}
On the other hand, the classical EOM is (here $e = 1$)
\begin{equation}
    \dot{\vb*{p}} = - \dot{\vb*{x}} \times \vb*{B}.
\end{equation}
So 
\begin{equation}
    \vb*{\Omega} = \Omega_0 \vu*{z}, \quad \Omega_0 = \frac{1}{B}.
\end{equation}

\item[6.] The size of the first Brillouin zone is 
\[
    \frac{(2\pi)^2}{2\pi / B} = 2\pi B.
\]
So 
\[
    2\pi C = \int \dd[2]{\vb*{k}} \Omega = 2\pi B \cdot \Omega_0 = 2\pi,
\]
and thus the Chern number of the Landau level is 1.

\end{itemize}

\end{document}