$$
\arctan (x) = \sum_{n=0}^\infty \frac{(-1)^n}{2n+1} x^{2n+1} = x - \frac{x^3}{3} + \frac{x^5}{5} - \ldots, \quad -1 < x < 1.
$$
$$
\arcsin (x) = x + \sum_{n=1}^\infty \frac{(2n-1)!!}{(2n)!!} \frac{x^{2n+1}}{2n+1} = x + \frac{x^3}{6} + \frac{3}{40}x^5 + \ldots, -1<x<1.
$$
$$
\frac{1}{\sqrt{1-x^2}} = \sum_{n=0}^\infty \frac{(2n-1)!!}{(2n)!!} x^{2n},
$$

$$
\ln (1+x) = \sum_{n\ge 1} \frac{(-1)^n x^n}{n}, \quad - \ln (1-x) = \sum_{n \ge 1} \frac{x^n}{n}.
$$

$$
2^n n! = (2n)!!, \quad \binom{-\frac{1}{2}}{n} = (-1)^n \frac{(2n-1)!!}{(2n)!!}.
$$
$$
\frac{1}{1-x} = \sum_{n=0}^\infty x^n = 1 + x + x^2 + \ldots, \\
\frac{x}{1-x} = \sum_{n=1}^\infty x^n = x + x^2 + x^3 + \ldots 
$$
$$
\frac{1}{(1-x)^2} = \sum_{n=0}^\infty (n+1)x^n = 1 + 2x + 3x^2 + \ldots, \\
\frac{x}{(1-x)^2} = \sum_{n=1}^\infty nx^n = \sum_{n=0}^\infty nx^n = x + 2x^2 + 3x^3 + \ldots
$$
